CM2_UMORTAL_dec.v
@@ -1,0 +1,156 @@
+Require Import List PeanoNat Lia Operators_Properties.
+Import ListNotations.
+
+Require Import ssreflect ssrbool ssrfun.
+Require Import M2.CM2 M2.CM2_facts.
+
+Section BoundConstruction.
+
+Variable M : Cm2.
+(* uniform bound *)
+Variable K : nat.
+Variable HK : forall x, bounded K M x.
+
+Notation step := (CM2.step M).
+Notation multi_step := (CM2.multi_step M).
+Notation mortal K := (CM2.mortal K M).
+
+Lemma bounded_inf k x : bounded k M x -> {L | (length L <= k) /\ (forall (y: Config), reaches M x y -> In y L) }.
+Proof.
+  move=> Hkx. exists (map (fun n => if multi_step n x is Some y then y else x) (seq 0 k)).
+  split; first by rewrite map_length seq_length.
+  move=> y Hxy. admit. (* hard, doable *)
+Admitted.
+
+Lemma pointwise_decision k x : (mortal k x) + (not (mortal k x)).
+Proof. rewrite /(mortal k). by case: (multi_step k x) => [y|]; [right|left]. Qed.
+
+Lemma pigeonhole {X : Type} (L L' : list X) : incl L L' -> length L' < length L -> not (NoDup L).
+Proof. Admitted.
+
+Lemma dup_seq {X : Type} (f : nat -> X) start len :
+  not (NoDup (map f (seq start len))) ->
+  exists '(i, j), f i = f j /\ (start <= i /\ i < j /\ j <= start+len).
+Proof.
+  elim: len start.
+  { move=> start /= H. exfalso. apply: H. by constructor. }
+  move=> len IH start /=.
+Admitted. 
+
+Lemma mortal_bound k x : mortal k x -> mortal K x.
+Proof.
+  rewrite /(mortal k). have [HkK|HKk] : k <= K \/ K < k by lia.
+  { move=> /multi_step_k_monotone. by apply. }
+  case Hxy: (multi_step K x) => [y|]; last done.
+  have [L [? HL]] := HK x.
+  have : incl (map (fun n => if multi_step n x is Some y then y else x) (seq 0 (K+1))) L.
+  { move=> z /in_map_iff [k'] [+ /in_seq ?].
+    case Hk': (multi_step k' x) => [z'|]; first last.
+    { move: Hk' => /(multi_step_k_monotone K) /(_ ltac:(lia)).
+      by rewrite Hxy. }
+    move=> <-. apply: HL. by exists k'. }
+  move=> /pigeonhole. rewrite map_length seq_length.
+  move=> /(_ ltac:(lia)) /dup_seq [[k1 k2]] [+ ?].
+  case Hk1: (multi_step k1 x) => [z|]; first last.
+  { admit. (* easy *) }
+  case Hk2: (multi_step k2 x) => [z'|]; first last.
+  { admit. (* easy *) }
+  move=> ?. subst z'.
+  admit. (* doable *)
+Admitted.
+
+Lemma pos_K : K = 1 + (K - 1).
+Proof.
+  suff: K <> 0 by lia.
+  move=> H'K.
+  have := HK (0, (0, 0)). rewrite H'K.
+  move=> [[|L]].
+  - by move=> [_] /(_ (0, (0, 0)) (reaches_refl _)).
+  - move=> ? /=. lia.
+Qed.
+
+Lemma mortal_K_bound_a {p a b} :
+  K <= a -> mortal K (p, (a, b)) <-> mortal K (p, (K, b)).
+Proof.
+  rewrite /(mortal _). elim: (K) p a b; first done.
+  move=> K' IH p a b Ha.
+  rewrite /= ?option_bind_iter /step -/step /=.
+  case: (nth_error M p) => [i|]; last done.
+  case: i.
+  - move=> c. rewrite -?/(multi_step _ _).
+    rewrite (IH _ (_ + a) (_ + b) ltac:(lia)).
+    by rewrite (IH _ (_ + (S K')) (_ + b) ltac:(lia)).
+  - move=> [] q.
+    + case: b => [|b].
+      * rewrite -?/(multi_step _ _).
+        rewrite (IH _ a 0 ltac:(lia)).
+        by rewrite (IH _ (S K') 0 ltac:(lia)).
+      * rewrite -?/(multi_step _ _).
+        rewrite (IH _ a b ltac:(lia)).
+        by rewrite (IH _ (S K') b ltac:(lia)).
+    + case: a Ha => [|a] Ha; first by lia.
+      rewrite -?/(multi_step _ _).
+      apply: IH. lia.
+Qed.
+
+Lemma mortal_K_bound_b {p a b} :
+  K <= b -> mortal K (p, (a, b)) <-> mortal K (p, (a, K)).
+Proof.
+Admitted.
+
+Lemma uniform_decision : (uniformly_mortal M) + (not (uniformly_mortal M)).
+Proof.
+  have := Forall_dec (fun 'x => mortal K x) _
+    (list_prod (seq 0 (length M)) (list_prod (seq 0 (K+1)) (seq 0 (K+1)))).
+  case.
+  { move=> x. rewrite /(mortal K). by case: (multi_step K x) => [y|]; [right|left]. }
+  - move=> H'M. left. exists K => - [p [a b]].
+    have [?|?] : length M <= p \/ p < length M by lia.
+    { rewrite /(mortal K) pos_K /multi_step iter_plus /= /step /=.
+      have -> : nth_error M p = None by apply /nth_error_None.
+      by rewrite iter_None. }
+    wlog ? : a /(a <= K).
+    { move=> H. (have [?|/mortal_K_bound_a] : a <= K \/ K <= a by lia); first by apply H.
+      move=> ->. by apply: H. }
+    wlog ? : b /(b <= K).
+    { move=> H. (have [?|/mortal_K_bound_b] : b <= K \/ K <= b by lia); first by apply H.
+      move=> ->. by apply: H. }
+    move: H'M => /Forall_forall. apply.
+    apply /in_prod.
+    { apply /in_seq. lia. }
+    apply /in_prod; apply /in_seq; lia.
+  - move=> H. right => - [K' H'M]. apply: H. apply /Forall_forall.
+    move=> [p [a b]] /in_prod_iff [/in_seq ?] /in_prod_iff [/in_seq ?] /in_seq ?.
+    by apply /mortal_bound /H'M.
+Qed.
+End BoundConstruction.
+
+
+
+Section BoundRefutation.
+
+Variable M : Cm2.
+Variable HM : not (uniformly_bounded M).
+
+Notation multi_step := (CM2.multi_step M).
+
+(* an unbounded machine is immortal *)
+Lemma not_uniformly_mortal : not (uniformly_mortal M).
+Proof.
+  move=> [k Hk]. apply: HM. exists k => x.
+  exists (map (fun n => if multi_step n x is Some y then y else x) (seq 0 k)).
+  split.
+  { rewrite map_length seq_length. lia. }
+  move=> y [k' Hk'].
+  have [?|?] : k' < k \/ k <= k' by lia.
+  - apply /in_map_iff. exists k'. rewrite Hk'.
+    split; first done. apply /in_seq. lia.
+  - have := Hk x. rewrite /mortal.
+    move=> /(multi_step_k_monotone k') /(_ ltac:(lia)).
+    by rewrite Hk'.
+Qed.
+
+End BoundRefutation.
+
+(* BoundConstruction decides uniform mortality knowing uniform bound
+BoundRefutation refutes uniform mortality with no uniform bound *)
